\documentclass{article}
\usepackage{epsfig}
\usepackage{amsmath}
\usepackage{xr}
\usepackage{amsfonts}
\pagestyle{empty}
\begin{document}
\[ \left( \begin{array}{cc} H & G^T \\ G & 0 \end{array} \right) \left( \begin{array}{c} \ddot{q} \\ - \lambda \end{array} \right) = \left( \begin{array}{c} -C + \tau \\ \gamma \end{array} \right) \]
\pagebreak

$H$
\pagebreak

$G$
\pagebreak

$C$
\pagebreak

$\gamma$
\pagebreak

\[ \left( \begin{array}{cc} H & G^T \\ G & 0 \end{array} \right) \left( \begin{array}{c} \dot{q}^{+} \\ \Lambda \end{array} \right) = \left( \begin{array}{c} H \dot{q}^{-} \\ v^{+} \end{array} \right) \]
\pagebreak

$\dot{q}^{+}$
\pagebreak

$\Lambda$
\pagebreak

$\dot{q}^{-}$
\pagebreak

$v^{+}$
\pagebreak

$\ddot{q}$
\pagebreak

$\lambda$
\pagebreak

$L^TL$
\pagebreak

\[ \left( \begin{array}{cc} H & G^T \\ G & 0 \end{array} \right) \left( \begin{array}{c} \ddot{q} \\ -\lambda \end{array} \right) = \left( \begin{array}{c} -C + \tau \\ \gamma \end{array} \right) \]
\pagebreak

$\Phi_{i,j}$
\pagebreak

\[ \left( \begin{array}{c} \dot{v}_1 \\ \dot{v}_2 \\ \vdots \\ \dot{v}_n \end{array} \right) = \left( \begin{array}{cccc} \Phi_{1,1} & \Phi_{1,2} & \cdots & \Phi{1,n} \\ \Phi_{2,1} & \Phi_{2,2} & \cdots & \Phi{2,n} \\ \cdots & \cdots & \cdots & \vdots \\ \Phi_{n,1} & \Phi_{n,2} & \cdots & \Phi{n,n} \end{array} \right) \left( \begin{array}{c} f_1 \\ f_2 \\ \vdots \\ f_n \end{array} \right) + \left( \begin{array}{c} \phi_1 \\ \phi_2 \\ \vdots \\ \phi_n \end{array} \right). \]
\pagebreak

$n$
\pagebreak

$\dot{v}_i$
\pagebreak

$f_i$
\pagebreak

$\phi_i$
\pagebreak

$ (n_\textit{dof} + n_c) \times (n_\textit{dof} + n_c$
\pagebreak

$ \mathbb{R}^{n_\textit{dof}}$
\pagebreak

$ \mathbb{R}^{n_c}$
\pagebreak

$n_\textit{dof} \times n_\textit{dof}$
\pagebreak

$\left[ \ Y \ | Z \ \right]$
\pagebreak

$GZ = 0$
\pagebreak

$\mathbb{R}^{n_\textit{dof}}$
\pagebreak

$ \ddot{q} = M(q)^{-1} ( -N(q, \dot{q}) + \tau)$
\pagebreak

$O(n_{dof})$
\pagebreak

$n_{dof}$
\pagebreak

\[ H \ddot{q} = -C + \tau \]
\pagebreak

$ \tau = M(q) \ddot{q} + N(q, \dot{q}) $
\pagebreak

$ M(q) $
\pagebreak

\[ (r_x, r_y, r_z, t_x, t_y, t_z) \]
\pagebreak

$x$
\pagebreak

$y$
\pagebreak

$z$
\pagebreak

$\mathbf{q}, \mathbf{\dot{q}}, \mathbf{\ddot{q}}$
\pagebreak

$\mathbf{\tau}$
\pagebreak

$\mathbf{q}$
\pagebreak

$q_i$
\pagebreak

$\mathbf{\dot{q}}$
\pagebreak

$\omega$
\pagebreak

$\mathbf{\ddot{q}}$
\pagebreak

$\dot{\omega}$
\pagebreak

$q$
\pagebreak

$\mathbf{\bar{q}}$
\pagebreak

$\mathbf{q},\mathbf{\bar{q}},\mathbf{\bar{\bar{q}}},\mathbf{\tau}$
\pagebreak

\begin{eqnarray*} \mathbf{q} &=& ( q_{tx}, q_{q1,x}, q_{q1,y}, q_{q1,z}, q_{ty}, q_{q2,x}, q_{q2,y}, q_{q2,z}, q_{q1,w}, q_{q2,w})^T \\ \mathbf{\bar{q}} &=& ( \dot{q}_{tx}, \omega_{1,x}, \omega_{1,y}, \omega_{1,z}, \dot{q}_{ty}, \omega_{2,x}, \omega_{2,y}, \omega_{2,z} )^T \\ \mathbf{\bar{\bar{q}}} &=& ( \ddot{q}_{tx}, \dot{\omega}_{1,x}, \dot{\omega}_{1,y}, \dot{\omega}_{1,z}, \ddot{q}_{ty}, \dot{\omega}_{2,x}, \dot{\omega}_{2,y}, \dot{\omega}_{2,z} )^T \\ \mathbf{\tau} &=& ( \tau_{tx}, \tau_{1,x}, \tau_{1,y}, \tau_{1,z}, \tau_{ty}, \tau_{2,x}, \tau_{2,y}, \tau_{2,z} )^T \end{eqnarray*}
\pagebreak

\[ q, \dot{q} \]
\pagebreak

$g(q(t))$
\pagebreak

$\frac{d}{dt} g(q(t)) = G(q)\dot{q}$
\pagebreak

$G(q)$
\pagebreak

${}^0 \hat{v}_i = G(q) * \dot{q}$
\pagebreak

\[ Qres = Qres + \Delta \theta\]
\pagebreak

\[ \Delta \theta = G^T (G^T G + \lambda^2 I)^{-1} e \]
\pagebreak

$G = G(q) = \frac{d}{dt} g(q(t))$
\pagebreak

$e$
\pagebreak

$||\Delta \theta||_2 \le$
\pagebreak

$\mathbf{\dot{q}}, \mathbf{\ddot{q}}$
\pagebreak

\[ X_{\lambda(i)} = {}^{i} X_{\lambda(i)} \]
\pagebreak

\end{document}
